\begin{figure}
	\begin{gather*}
     	\begin{aligned}
    	\mathrm{path} \; \defeq \; &(\m{v}_0, [e_0, e_1, \dots, e_k]) \\ 
    	\mathtt{s\_evalid}(\gamma, e) \; \defeq \; & \mathtt{E}_{\gamma}(e) /| 
    	\mathtt{V}_{\gamma}(\mathtt{src}_{\gamma}(e)) /| 
    	\mathtt{V}_{\gamma}(\mathtt{dst}_{\gamma}(e)) \\
		\mathtt{valid\_path}\big(\gamma, (\m{v},[])\big) \;\defeq \; & \mathtt{V}_{\gamma}(\m{v})\\
		\mathtt{valid\_path}\big(\gamma, (\m{v},[e_1,e_2,\dots,e_n])\big) \; \defeq \; &\m{v}=\mathtt{src}_{\gamma}(e_1) \wedge \mathtt{s\_evalid}(\gamma,e_1) \wedge \null \\
    &\mathtt{dst}_{\gamma}(e_1)=\mathtt{src}_{\gamma}(e_2) \wedge \null\\
    &\mathtt{s\_evalid}(\gamma, e_2) \wedge \dots /| \mathtt{dst}_{\gamma}(e_{n-1})=\mathtt{src}_{\gamma}(e_n) \\ 
        \mathtt{end}\big(\gamma, (\m{v}, [])\big)\;\defeq\;& \m{v}\\
      	\mathtt{end}\big(\gamma, (\m{v},[e_1,e_2,\dots,e_n])\big)\;\defeq\;&
      	\mathtt{dst}_{\gamma}(e_{n})\\
      	\gamma \vDash s \overset{\m{p}}{\leadsto} t \;\defeq\; &
        \mathtt{valid\_path}(\gamma, p)\wedge
        \mathtt{fst}(p)=s \wedge \mathtt{end}(\gamma,p)=t \\
        \gamma_1 \cong \gamma_2 \; \defeq \; & 
        	\forall e.~\mathtt{E}_{\gamma_1}(e) <=> \mathtt{E}_{\gamma_2}(e) /| \forall \m{v}.~\mathtt{V}_{\gamma_1}(\m{v}) <=> \mathtt{V}_{\gamma_1}(\m{v}) /| \null \\
        	&\forall e.~\mathtt{E}_{\gamma_1}(e) ==> \mathtt{src}_{\gamma_1}(e) = \mathtt{src}_{\gamma_2}(e) /| \mathtt{dst}_{\gamma_1}(e) = \mathtt{dst}_{\gamma_2}(e) \\
       	\gamma \smallsetminus S \; \defeq \; 
       	 	&{\mathcal{V}}_{\gamma'} = {\mathcal{V}}_{\gamma} /| 
          {\mathcal{E}}_{\gamma'} = {\mathcal{E}}_{\gamma} /| \null \\
          &{\mathtt{src}}_{\gamma'} = {\mathtt{src}}_{\gamma} /|
          {\mathtt{dst}}_{\gamma'} = {\mathtt{dst}}_{\gamma} /| \null \\
       	 	&\gamma'_{\mathtt{V}} = \Big(\lambda x.~ \gamma_{\mathtt{V}}(x) /| \lnot S_{\mathtt{V}}(x)\Big) /| \null \\ 
       	 	&\gamma'_{\mathtt{E}} = \Big(\lambda x.~ \gamma_{\mathtt{E}}(x) /| \lnot S_{\mathtt{E}}(x)\Big)\\
%        	\begin{minipage}[c]{.5\linewidth} \hline \end{minipage}
        \mathrm{MathGraph}(\gamma)\,\defeq\,\Big\{
          \mathtt{null}:\; & V\\ 
          \mathtt{valid\_graph}:\;& \forall e\,.\,\mathtt{evalid}(\gamma, e) \Rightarrow
          \mathtt{vvalid}\big(\gamma, \mathtt{src}(\gamma, e)\big)\wedge \null \\
          & \qquad \big(\m{e} = \mathtt{null} \vee \mathtt{vvalid}(\gamma, \m{e})\big)\\
          \mathtt{valid\_not\_null}:\;& \forall \m{v}\,.\,\mathtt{vvalid}(\gamma, \m{v})
          \Rightarrow \m{v} \neq \mathtt{null} \Big\} \\
        \mathrm{LstGraph}(\gamma)\,\defeq\, \Big\{
          \mathtt{out}:\; & V \rightarrow E\\
          \mathtt{only\_one\_edge}:\; & \forall \m{v},\,e\,.\,
          \mathtt{vvalid}(\gamma, \m{v}) \Rightarrow \\
          & \Big(\mathtt{src}(\gamma, e) =\m{v} \wedge
          \mathtt{evalid}(\gamma, e)\Big) \Leftrightarrow
          e = \mathtt{out}(\m{v})\\
         \mathtt{acyclic\_path}:\; & \forall \m{v},\,p\,.\,
         \gamma \vDash \m{v} \overset{p}{\leadsto} \m{v} \Rightarrow p = (\m{v},[])\Big\} \\
       	\mathrm{FiniteGraph}(\gamma)\,\defeq\, \Big\{
          \mathtt{finite\_\m{v}}:\;&\exists\, S_\m{v},\, M_\m{v}\;\text{s.t.}\;\lvert S_\m{v}\rvert
          \leq M_\m{v} \wedge
          \forall \m{v}\,.\, \mathtt{vvalid}(\gamma,\m{v})\Rightarrow \m{v}\,\in\,S_\m{v}\\
          \mathtt{finite\_e}:\;&\exists\, S_e,\, M_e\;\text{s.t.}\;\lvert S_e\rvert
          \leq M_e \wedge
          \forall e\,.\, \mathtt{evalid}(\gamma,e)\Rightarrow e\,\in\,S_e \Big\}
    	\end{aligned}
    \end{gather*}
\caption{Some Graph definitions}
\label{fig:graphdefns}
\vspace{-1em}
\end{figure}