\documentclass{article}
\usepackage[a4paper,left=1.5cm,right=1.5cm,bottom=2.5cm,top=2.5cm]{geometry}
\usepackage[tbtags]{amsmath} %\usepackage{amsmath}
\usepackage{mathtools}
\usepackage{mathpartir}
\usepackage{amssymb}
\usepackage{mathabx}
\usepackage{listings}          % format code
\usepackage{xcolor}   % hyperli
\usepackage{semantic}
\newcommand{\tx}[1]{\text{#1}}
\newcommand{\p}[1]{\ensuremath{\mathsf{#1}}} % predicate font
\newcommand{\m}[1]{\ensuremath{\mathit{#1}}} % math font
\newcommand{\scon}{\mathbin{\varstar}}
\newcommand{\ocon}{%
  \mathbin{\mbox{$\mathrlap{\cup}\hspace*{.15em}
      \raisebox{.01em}[0ex][0ex]{$\scon$}$\hspace*{.07em}}}}
\newcommand{\wand}{%
 \mathrel{\mbox{$\hspace*{-0.03em}\mathord{-}\hspace*{-0.66em}
     \mathord{-}\hspace*{-0.36em}\mathord{\scon}$\hspace*{-0.005em}}}}
\newcommand{\septraction}{%
  \mathrel{\mbox{$\hspace*{-0.03em}\mathord{-}\hspace*{-0.66em}
  \mathord{-}\hspace*{-0.155em}\mathord{\ocircle\hspace*{-.66em}\scon}$\hspace*{0.05em}}}}
\newcommand{\magicwand}{\wand}
\lstset{%
  language=C,
  morecomment=[n][{\color{red!80!black}}]{/*}{*/},
  morecomment=[l][{\color{red!80!black}}]{//},
  sensitive=true,
  mathescape=true,
  showlines=true,
  basicstyle=\normalfont\small\tt,
  keywordstyle=\color{blue},
  numbers=left,
  numberstyle=\tiny,
  numbersep=5pt,
  boxpos=t,
}

\mathlig{--*}{\mathrel{\magicwand}}
\mathlig{--o}{\mathrel{\septraction}}
\mathlig{|->}{\mathrel{\mapsto}} % tight points-to
\mathlig{<=>}{\mathrel{\Leftrightarrow}} % equivalence of expressions
\mathlig{==>}{\mathrel{\Rightarrow}} % meta implication
\mathlig{-|-}{\mathrel{\mathrlap{\dashv} \hspace{5pt} \vdash}} % entails
\mathlig{/|}{\mathbin{\wedge}} % additive conjunction
\mathlig{|/}{\mathbin{\vee}} % additive disjunction
\mathlig{|-}{\mathrel{\vdash}} % entails
\mathlig{|=}{\vDash} % models
\mathlig{**}{\mathbin{\ocon}}
\mathlig{*}{\mathbin{\scon}}

\begin{document}

The following is the old proof:

\begin{figure}[t]
\begin{lstlisting}
struct Node {
    int m;
    struct Node * l;
    struct Node * r; };

// We use $R$ to represent $\p{reachable}(\gamma,\tx x)$

void spanning(struct Node * x) {// $\{\p{graph}(\tx{x},\gamma)/|\gamma(\tx{x}).1=0\}$
    struct Node * l, * r; int root_mark;
// $\{\p{graph}(\tx x,\gamma) /| \exists l,r.~ \gamma(\tx{x}) = (0,l,r)\}$
// $\{\p{graph}(\tx x,\gamma) /| \gamma(\tx{x}) = (0,l,r)\}$
// $\{\p{vertices\_at}(\p{reachable}(\gamma,\tx x), \gamma) /| \gamma(\tx{x}) = (0,l,r)\}$
// $\{\p{vertices\_at}(R, \gamma) /| \gamma(\tx{x}) = (0,l,r)\}$
// $\searrow \{\tx x|-> 0,l,r /| \gamma(\tx{x}) = (0,l,r)\}$
    l = x -> l;
    r = x -> r;
    x -> m = 1;
// $\swarrow \{\tx x|-> 1,\tx{l},\tx{r} /| \gamma(\tx{x}) = (0,\tx{l},\tx{r}) /| \exists \gamma_1.~ \m{mark1}(\gamma, \tx{x}, \gamma_1)\}$
// $\{\exists \gamma_1.~\p{vertices\_at}(R, \gamma_1) /| \gamma(\tx{x}) = (0,\tx{l},\tx{r}) /| \m{mark1}(\gamma, \tx{x}, \gamma_1)\}$
// $\{\p{vertices\_at}(R, \gamma_1) /| \gamma(\tx{x}) = (0,\tx{l},\tx{r}) /| \m{mark1}(\gamma, \tx{x}, \gamma_1)\}$
    if (l) {
        root_mark = l -> m;
        if (root_mark == 0) {
            spanning(l);
        } else { x -> l = 0; } }
// $\left\{\!\!\!\begin{array}{l@{}}\exists\gamma_2. ~\p{vertices\_at}(R,\gamma_2)/| \gamma(\tx{x}) = (0,\tx{l},\tx{r})  /| \null \\ \m{mark1}(\gamma, \tx{x}, \gamma_1) /| \m{e\_span}(\gamma_1,\tx{x}.\text{L},\gamma_2)\end{array}\right\}$
// $\left\{\!\!\!\begin{array}{l@{}}\p{vertices\_at}(R,\gamma_2)/| \gamma(\tx{x}) = (0,\tx{l},\tx{r})  /| \null \\ \m{mark1}(\gamma, \tx{x}, \gamma_1) /|  \m{e\_span}(\gamma_1,\tx{x}.\text{L},\gamma_2)\end{array}\right\}$
    if (r) {
        root_mark = r -> m;
        if (root_mark == 0) {
           spanning(r);
        } else { x -> r = 0; } }
// $\left\{\!\!\!\begin{array}{l@{}}\exists\gamma_3.~\p{vertices\_at}(R,\gamma_3)/| \gamma(\tx{x}) = (0,\tx{l},\tx{r})  /| \null \\ \m{mark1}(\gamma, \tx{x}, \gamma_1) /| \m{e\_span}(\gamma_1,\tx{x}.\text{L},\gamma_2) /| \m{e\_span}(\gamma_2,\tx{x}.\text{R},\gamma_3)\end{array}\right\}$
} // $\{\exists \gamma_3.~\p{vertex\_at}(\p{reachable}(\gamma, \tx{x}), \gamma_3)/|\m{span}(\gamma,\tx{x},\gamma_3)\}$
\end{lstlisting}
\caption{Old proof}
\end{figure}

\begin{figure}[t]
\begin{lstlisting}
struct Node {
    int m;
    struct Node * l;
    struct Node * r; };

void spanning(struct Node * x) {// $\{\p{graph}(\tx{x},\gamma)/|\gamma(\tx{x}).1=0\}$
    struct Node * l, * r; int root_mark;
// $\{\p{graph}(\tx x,\gamma) /| \exists l,r.~ \gamma(\tx{x}) = (0,l,r)\}$
// $\{\p{graph}(\tx x,\gamma) /| \gamma(\tx{x}) = (0,l,r)\}$
// $\searrow \{\tx x|-> 0,l,r /| \gamma(\tx{x}) = (0,l,r)\}$
    l = x -> l;
    r = x -> r;
    x -> m = 1;
// $\swarrow \{\tx x|-> 1,\tx{l},\tx{r} /| \gamma(\tx{x}) = (0,\tx{l},\tx{r}) /| \exists \gamma_1.~ \m{mark1}(\gamma, \tx{x}, \gamma_1)\}$
// $\{\exists \gamma_1.~\p{graph}(\tx x, \gamma_1) /| \gamma(\tx{x}) = (0,\tx{l},\tx{r}) /| \m{mark1}(\gamma, \tx{x}, \gamma_1)\}$
// $\{\p{graph}(\tx x, \gamma_1) /| \gamma(\tx{x}) = (0,\tx{l},\tx{r}) /| \m{mark1}(\gamma, \tx{x}, \gamma_1)\}$
    if (l) {
// $\{\p{graph}(\tx x, \gamma_1) /| \gamma(\tx{x}) = (0,\tx{l},\tx{r}) /| \exists m_2, l_2, r_2.~\gamma_1(\tx{l})=(m_2, l_2, r_2) /| \m{mark1}(\gamma, \tx{x}, \gamma_1)\}$
// $\{\p{graph}(\tx x, \gamma_1) /| \gamma(\tx{x}) = (0,\tx{l},\tx{r}) /| \gamma_1(\tx{l})=(m_2, l_2, r_2) /| \m{mark1}(\gamma, \tx{x}, \gamma_1)\}$
// $\searrow\{\tx{l} |-> m_2, -, l_2, r_2\}$
        root_mark = l -> m;
// $\swarrow\{\tx{l} |-> m_2, -, l_2, r_2/|m_2 = \tx{root\_mark}\}$
// $\{\p{graph}(\tx x, \gamma_1)/| \gamma(\tx{x}) = (0,\tx{l},\tx{r})/|\gamma_1(\tx{l})=(m_2, l_2, r_2)/|m_2 = \tx{root\_mark} /| \m{mark1}(\gamma, \tx{x}, \gamma_1)\}$
        if (root_mark == 0) {
// $\{\p{graph}(\tx x, \gamma_1)/|\gamma(\tx{x}) = (0,\tx{l},\tx{r})/|\gamma_1(\tx{l})=(0, l_2, r_2) /| \m{mark1}(\gamma, \tx{x}, \gamma_1)\}$
// $\searrow\{\p{graph}(\tx{l}, \gamma_1)/|\gamma_1(\tx{l})=(0, l_2, r_2)\}$
            spanning(l);
// $\swarrow\{\exists \gamma_2. ~\p{graph}(\tx l, \gamma_2)/|\gamma_1(\tx{l})=(0, l_2, r_2)/|\m{span}(\gamma_1,\tx{l},\gamma_2)\}$
// $\{\exists \gamma_2. ~\p{graph}(\tx x, \gamma_2)/|\gamma(\tx{x}) = (0,\tx{l},\tx{r}) /|\gamma_1(\tx{l})=(0, l_2, r_2) /| \m{mark1}(\gamma, \tx{x}, \gamma_1) /|\m{span}(\gamma_1,\tx{l},\gamma_2)\}$
        } else { // $\{\p{graph}(\tx x, \gamma_1)/| \gamma(\tx{x}) = (0,\tx{l},\tx{r})/|\gamma_1(\tx{l})=(1, l_2, r_2)  /| \m{mark1}(\gamma, \tx{x}, \gamma_1)\}$
// $\searrow \{\tx x|-> 0,\tx{l},\tx{r} /| \gamma(\tx{x}) = (0,\tx{l},\tx{r})\}$
          x -> l = 0;
// $\swarrow \{\tx x|-> 0,0,\tx{r} /| \gamma(\tx{x}) = (0,\tx{l},\tx{r})\}$
// $\{\exists \gamma_2. ~\p{graph}(\tx x, \gamma_2)/|\gamma(\tx{x}) = (0,\tx{l},\tx{r})/|\gamma_1(\tx{l})=(1, l_2, r_2) /| \m{mark1}(\gamma, \tx{x}, \gamma_1) /| \m{cut}(\gamma_1, l, \gamma_2)\}$
        } // $\{\exists\gamma_2.~\p{graph}(\tx x,\gamma_2)/| \gamma(\tx{x}) = (0,\tx{l},\tx{r})  /| \m{mark1}(\gamma, \tx{x}, \gamma_1) /| \m{e\_span}(\gamma_1,\tx{x}.\text{L},\gamma_2)\}$
    } else { // $\{\p{graph}(\tx x, \gamma_1) /| \gamma(\tx{x}) = (0,\tx{l},\tx{r}) /| \tx{l}= 0  /| \m{mark1}(\gamma, \tx{x}, \gamma_1)\}$
      skip;
// $\{\exists\gamma_2. ~\p{graph}(\tx x,\gamma_2)/| \gamma(\tx{x}) = (0,\tx{l},\tx{r})  /| \m{mark1}(\gamma, \tx{x}, \gamma_1) /| \m{e\_span}(\gamma_1,\tx{x}.\text{L},\gamma_2)\}$
    } // $\{\exists\gamma_2. ~\p{graph}(\tx x,\gamma_2)/| \gamma(\tx{x}) = (0,\tx{l},\tx{r})  /| \m{mark1}(\gamma, \tx{x}, \gamma_1) /| \m{e\_span}(\gamma_1,\tx{x}.\text{L},\gamma_2)\}$
// $\{\p{graph}(\tx x,\gamma_2)/| \gamma(\tx{x}) = (0,\tx{l},\tx{r})  /| \m{mark1}(\gamma, \tx{x}, \gamma_1) /|  \m{e\_span}(\gamma_1,\tx{x}.\text{L},\gamma_2)\}$
    if (r) {
// $\{\p{graph}(\tx x, \gamma_2) /| \gamma(\tx{x}) = (0,\tx{l},\tx{r}) /| \exists m_2, l_2, r_2.~\gamma_1(\tx{l})=(m_2, l_2, r_2) /| \m{mark1}(\gamma, \tx{x}, \gamma_1)/| \m{e\_span}(\gamma_1,\tx{x}.\text{L},\gamma_2)\}$
// $\{\p{graph}(\tx x, \gamma_2) /| \gamma(\tx{x}) = (0,\tx{l},\tx{r}) /| \gamma_2(\tx{r})=(m_2, l_2, r_2) /| \m{mark1}(\gamma, \tx{x}, \gamma_1)/| \m{e\_span}(\gamma_1,\tx{x}.\text{L},\gamma_2)\}$
// $\searrow\{\tx{r} |-> m_2, -, l_2, r_2\}$
        root_mark = r -> m;
// $\swarrow\{\tx{r} |-> m_2, -, l_2, r_2/|m_2 = \tx{root\_mark}\}$
// $\{\p{graph}(\tx x, \gamma_2)/| \gamma(\tx{x}) = (0,\tx{l},\tx{r})/|\gamma_2(\tx{r})=(m_2, l_2, r_2)/|m_2 = \tx{root\_mark} /| \m{mark1}(\gamma, \tx{x}, \gamma_1)/| \m{e\_span}(\gamma_1,\tx{x}.\text{L},\gamma_2)\}$
        if (root_mark == 0) {
// $\{\p{graph}(\tx x, \gamma_2)/|\gamma(\tx{x}) = (0,\tx{l},\tx{r})/|\gamma_2(\tx{r})=(0, l_2, r_2) /| \m{mark1}(\gamma, \tx{x}, \gamma_1)/| \m{e\_span}(\gamma_1,\tx{x}.\text{L},\gamma_2)\}$
// $\searrow\{\p{graph}(\tx{r}, \gamma_2)/|\gamma_2(\tx{r})=(0, l_2, r_2)\}$
           spanning(r);
// $\swarrow\{\exists \gamma_3. ~\p{graph}(\tx r, \gamma_3)/|\gamma_2(\tx{r})=(0, l_2, r_2)/|\m{span}(\gamma_2,\tx{r},\gamma_3)\}$
// $\{\exists \gamma_3. ~\p{graph}(\tx x, \gamma_3)/|\gamma(\tx{x}) = (0,\tx{l},\tx{r}) /|\gamma_2(\tx{r})=(0, l_2, r_2) /| \m{mark1}(\gamma, \tx{x}, \gamma_1) /|\m{span}(\gamma_1,\tx{l},\gamma_2)/|\m{span}(\gamma_2,\tx{r},\gamma_3)\}$
        } else { // $\{\p{graph}(\tx x, \gamma_2)/| \gamma(\tx{x}) = (0,\tx{l},\tx{r})/|\gamma_2(\tx{r})=(1, l_2, r_2)  /| \m{mark1}(\gamma, \tx{x}, \gamma_1) /| \m{e\_span}(\gamma_1,\tx{x}.\text{L},\gamma_2)\}$
// $\searrow \{\tx x|-> 0,?l,\tx{r} /| \gamma(\tx{x}) = (0,?l,\tx{r})\}$
            x -> r = 0;
// $\swarrow \{\tx x|-> 0,?l,\tx{r} /| \gamma(\tx{x}) = (0,?l,\tx{r})\}$
// $\{\exists \gamma_3. ~\p{graph}(\tx x, \gamma_3)/|\gamma(\tx{x}) = (0,\tx{l},\tx{r})/|\gamma_2(\tx{r})=(1, l_2, r_2) /| \m{mark1}(\gamma, \tx{x}, \gamma_1) /| \m{e\_span}(\gamma_1,\tx{x}.\text{L},\gamma_2) /| \m{cut}(\gamma_2, r, \gamma_3)\}$
        } // $\{\exists\gamma_3.~\p{graph}(\tx x,\gamma_3)/| \gamma(\tx{x}) = (0,\tx{l},\tx{r})  /| \m{mark1}(\gamma, \tx{x}, \gamma_1) /| \m{e\_span}(\gamma_1,\tx{x}.\text{L},\gamma_2) /| \m{e\_span}(\gamma_2,\tx{x}.\text{R},\gamma_3)\}$
    } else { // $\{\p{graph}(\tx x, \gamma_2) /| \gamma(\tx{x}) = (0,\tx{l},\tx{r}) /| \tx{r}= 0  /| \m{mark1}(\gamma, \tx{x}, \gamma_1)  /| \m{e\_span}(\gamma_1,\tx{x}.\text{L},\gamma_2)\}$
        skip;
// $\{\exists\gamma_3.~\p{graph}(\tx x,\gamma_3)/| \gamma(\tx{x}) = (0,\tx{l},\tx{r})  /| \m{mark1}(\gamma, \tx{x}, \gamma_1) /| \m{e\_span}(\gamma_1,\tx{x}.\text{L},\gamma_2) /| \m{e\_span}(\gamma_2,\tx{x}.\text{R},\gamma_3)\}$
    } // $\{\exists\gamma_3.~\p{graph}(\tx x,\gamma_3)/| \gamma(\tx{x}) = (0,\tx{l},\tx{r})  /| \m{mark1}(\gamma, \tx{x}, \gamma_1) /| \m{e\_span}(\gamma_1,\tx{x}.\text{L},\gamma_2) /| \m{e\_span}(\gamma_2,\tx{x}.\text{R},\gamma_3)\}$
} // $\{\exists \gamma_3.~\p{graph}(\tx x, \gamma_3)/|\m{span}(\gamma,\tx{x},\gamma_3)\}$
\end{lstlisting}
\caption{new proof}
\end{figure}

\end{document}

