\begin{figure*}
  \begin{lstlisting}
struct Node {
    int m;
    struct Node * l;
    struct Node * r; };

// We use $R$ to represent $\p{reachable}(\gamma,\tx x)$

void spanning(struct Node * x) { // $\{\p{graph}(\tx{x},\gamma)/|\gamma(\tx{x}).1=0\}$
    struct Node * l, * r; int root_mark;
// $\{\p{graph}(\tx x,\gamma) /| \exists l,r.~ \gamma(\tx{x}) = (0,l,r)\}$
// $\{\p{graph}(\tx x,\gamma) /| \gamma(\tx{x}) = (0,l,r)\}$
// $\{\p{vertices\_at}(\p{reachable}(\gamma,\tx x), \gamma) /| \gamma(\tx{x}) = (0,l,r)\}$
// $\{\p{vertices\_at}(R, \gamma) /| \gamma(\tx{x}) = (0,l,r)\}$
// $\searrow \{\tx x|-> 0,l,r /| \gamma(\tx{x}) = (0,l,r)\}$
    l = x -> l; r = x -> r; x -> m = 1;
// $\swarrow \{\tx x|-> 1,\tx{l},\tx{r} /| \gamma(\tx{x}) = (0,\tx{l},\tx{r}) /| \exists \gamma_1.~ \m{mark1}(\gamma, \tx{x}, \gamma_1)\}$
// $\{\exists \gamma_1.~\p{vertices\_at}(R, \gamma_1) /| \gamma(\tx{x}) = (0,\tx{l},\tx{r}) /| \m{mark1}(\gamma, \tx{x}, \gamma_1)\}$
// $\{\p{vertices\_at}(R, \gamma_1) /| \gamma(\tx{x}) = (0,\tx{l},\tx{r}) /| \m{mark1}(\gamma, \tx{x}, \gamma_1)\}$
    if (l) {
// $\{\p{vertices\_at}(R, \gamma_1) /| \gamma(\tx{x}) = (0,\tx{l},\tx{r}) /| \exists m_2, l_2, r_2.~\gamma_1(\tx{l})=(m_2, l_2, r_2) /| \m{mark1}(\gamma, \tx{x}, \gamma_1)\}$
// $\{\p{vertices\_at}(R, \gamma_1) /| \gamma(\tx{x}) = (0,\tx{l},\tx{r}) /| \gamma_1(\tx{l})=(m_2, l_2, r_2) /| \m{mark1}(\gamma, \tx{x}, \gamma_1)\}$
// $\searrow\{\tx{l} |-> m_2, -, l_2, r_2\}$
        root_mark = l -> m;
// $\swarrow\{\tx{l} |-> m_2, -, l_2, r_2/|m_2 = \tx{root\_mark}\}$
// $\{\p{vertices\_at}(R, \gamma_1)/| \gamma(\tx{x}) = (0,\tx{l},\tx{r})/|\gamma_1(\tx{l})=(m_2, l_2, r_2)/|m_2 = \tx{root\_mark} /| \m{mark1}(\gamma, \tx{x}, \gamma_1)\}$
        if (root_mark == 0) {
// $\{\p{vertices\_at}(R, \gamma_1)/|\gamma(\tx{x}) = (0,\tx{l},\tx{r})/|\gamma_1(\tx{l})=(0, l_2, r_2) /| \m{mark1}(\gamma, \tx{x}, \gamma_1)\}$
// $\searrow\{\p{graph}(\tx{l}, \gamma_1)/|\gamma_1(\tx{l})=(0, l_2, r_2)\}$
            spanning(l);
// $\swarrow\{\exists \gamma_2. ~\p{vertices\_at}(\p{reachable}(\gamma_1,\tx l), \gamma_2)/|\gamma_1(\tx{l})=(0, l_2, r_2)/|\m{span}(\gamma_1,\tx{l},\gamma_2)\}$
// $\{\exists \gamma_2. ~\p{vertices\_at}(R, \gamma_2)/|\gamma(\tx{x}) = (0,\tx{l},\tx{r}) /|\gamma_1(\tx{l})=(0, l_2, r_2) /| \m{mark1}(\gamma, \tx{x}, \gamma_1) /|\m{span}(\gamma_1,\tx{l},\gamma_2)\}$
        } else { // $\{\p{vertices\_at}(R, \gamma_1)/| \gamma(\tx{x}) = (0,\tx{l},\tx{r})/|\gamma_1(\tx{l})=(1, l_2, r_2)  /| \m{mark1}(\gamma, \tx{x}, \gamma_1)\}$
// $\searrow \{\tx x|-> 0,\tx{l},\tx{r} /| \gamma(\tx{x}) = (0,\tx{l},\tx{r})\}$
            x -> l = 0;
// $\swarrow \{\tx x|-> 0,0,\tx{r} /| \gamma(\tx{x}) = (0,\tx{l},\tx{r})\}$
// $\{\exists \gamma_2. ~\p{vertices\_at}(R, \gamma_2)/|\gamma(\tx{x}) = (0,\tx{l},\tx{r})/|\gamma_1(\tx{l})=(1, l_2, r_2) /| \m{mark1}(\gamma, \tx{x}, \gamma_1) /| \m{e\_rm}(\gamma_1, \tx{x}.\text{L}, \gamma_2)\}$
        } // $\{\exists\gamma_2.~\p{vertices\_at}(R,\gamma_2)/| \gamma(\tx{x}) = (0,\tx{l},\tx{r})  /| \m{mark1}(\gamma, \tx{x}, \gamma_1) /| \m{e\_span}(\gamma_1,\tx{x}.\text{L},\gamma_2)\}$
    }
    else { // $\{\p{vertices\_at}(R, \gamma_1) /| \gamma(\tx{x}) = (0,\tx{l},\tx{r}) /| \tx{l}= 0  /| \m{mark1}(\gamma, \tx{x}, \gamma_1)\}$
        skip;
// $\{\exists\gamma_2. ~\p{vertices\_at}(R,\gamma_2)/| \gamma(\tx{x}) = (0,\tx{l},\tx{r})  /| \m{mark1}(\gamma, \tx{x}, \gamma_1) /| \m{e\_span}(\gamma_1,\tx{x}.\text{L},\gamma_2)\}$
    } // $\{\exists\gamma_2. ~\p{vertices\_at}(R,\gamma_2)/| \gamma(\tx{x}) = (0,\tx{l},\tx{r})  /| \m{mark1}(\gamma, \tx{x}, \gamma_1) /| \m{e\_span}(\gamma_1,\tx{x}.\text{L},\gamma_2)\}$
// $\{\p{vertices\_at}(R,\gamma_2)/| \gamma(\tx{x}) = (0,\tx{l},\tx{r})  /| \m{mark1}(\gamma, \tx{x}, \gamma_1) /|  \m{e\_span}(\gamma_1,\tx{x}.\text{L},\gamma_2)\}$
    if (r) {
// $\{\p{vertices\_at}(R, \gamma_2) /| \gamma(\tx{x}) = (0,\tx{l},\tx{r}) /| \exists m_2, l_2, r_2.~\gamma_1(\tx{l})=(m_2, l_2, r_2) /| \m{mark1}(\gamma, \tx{x}, \gamma_1)/| \m{e\_span}(\gamma_1,\tx{x}.\text{L},\gamma_2)\}$
// $\{\p{vertices\_at}(R, \gamma_2) /| \gamma(\tx{x}) = (0,\tx{l},\tx{r}) /| \gamma_2(\tx{r})=(m_2, l_2, r_2) /| \m{mark1}(\gamma, \tx{x}, \gamma_1)/| \m{e\_span}(\gamma_1,\tx{x}.\text{L},\gamma_2)\}$
// $\searrow\{\tx{r} |-> m_2, -, l_2, r_2\}$
        root_mark = r -> m;
// $\swarrow\{\tx{r} |-> m_2, -, l_2, r_2/|m_2 = \tx{root\_mark}\}$
// $\{\p{vertices\_at}(R, \gamma_2)/| \gamma(\tx{x}) = (0,\tx{l},\tx{r})/|\gamma_2(\tx{r})=(m_2, l_2, r_2)/|m_2 = \tx{root\_mark} /| \m{mark1}(\gamma, \tx{x}, \gamma_1)/| \m{e\_span}(\gamma_1,\tx{x}.\text{L},\gamma_2)\}$
        if (root_mark == 0) {
// $\{\p{vertices\_at}(R, \gamma_2)/|\gamma(\tx{x}) = (0,\tx{l},\tx{r})/|\gamma_2(\tx{r})=(0, l_2, r_2) /| \m{mark1}(\gamma, \tx{x}, \gamma_1)/| \m{e\_span}(\gamma_1,\tx{x}.\text{L},\gamma_2)\}$
// $\searrow\{\p{graph}(\tx{r}, \gamma_2)/|\gamma_2(\tx{r})=(0, l_2, r_2)\}$
           spanning(r);
// $\swarrow\{\exists \gamma_3. ~\p{vertices\_at}(\p{reachable}(\gamma_2,\tx r), \gamma_3)/|\gamma_2(\tx{r})=(0, l_2, r_2)/|\m{span}(\gamma_2,\tx{r},\gamma_3)\}$
// $\{\exists \gamma_3. ~\p{vertices\_at}(R, \gamma_3)/|\gamma(\tx{x}) = (0,\tx{l},\tx{r}) /|\gamma_2(\tx{r})=(0, l_2, r_2) /| \m{mark1}(\gamma, \tx{x}, \gamma_1) /|\m{span}(\gamma_1,\tx{l},\gamma_2)/|\m{span}(\gamma_2,\tx{r},\gamma_3)\}$
        } else { // $\{\p{vertices\_at}(R, \gamma_2)/| \gamma(\tx{x}) = (0,\tx{l},\tx{r})/|\gamma_2(\tx{r})=(1, l_2, r_2)  /| \m{mark1}(\gamma, \tx{x}, \gamma_1) /| \m{e\_span}(\gamma_1,\tx{x}.\text{L},\gamma_2)\}$
// $\searrow \{\tx x|-> 0,?l,\tx{r} /| \gamma(\tx{x}) = (0,?l,\tx{r})\}$
            x -> r = 0;
// $\swarrow \{\tx x|-> 0,?l,\tx{r} /| \gamma(\tx{x}) = (0,?l,\tx{r})\}$
// $\{\exists \gamma_3. ~\p{vertices\_at}(R, \gamma_3)/|\gamma(\tx{x}) = (0,\tx{l},\tx{r})/|\gamma_2(\tx{r})=(1, l_2, r_2) /| \m{mark1}(\gamma, \tx{x}, \gamma_1) /| \m{e\_span}(\gamma_1,\tx{x}.\text{L},\gamma_2) /| \m{e\_rm}(\gamma_2, \tx{x}.\text{R}, \gamma_3)\}$
        } // $\{\exists\gamma_3.~\p{vertices\_at}(R,\gamma_3)/| \gamma(\tx{x}) = (0,\tx{l},\tx{r})  /| \m{mark1}(\gamma, \tx{x}, \gamma_1) /| \m{e\_span}(\gamma_1,\tx{x}.\text{L},\gamma_2) /| \m{e\_span}(\gamma_2,\tx{x}.\text{R},\gamma_3)\}$
    } else { // $\{\p{vertices\_at}(R, \gamma_2) /| \gamma(\tx{x}) = (0,\tx{l},\tx{r}) /| \tx{r}= 0  /| \m{mark1}(\gamma, \tx{x}, \gamma_1)  /| \m{e\_span}(\gamma_1,\tx{x}.\text{L},\gamma_2)\}$
        skip;
// $\{\exists\gamma_3.~\p{vertices\_at}(R,\gamma_3)/| \gamma(\tx{x}) = (0,\tx{l},\tx{r})  /| \m{mark1}(\gamma, \tx{x}, \gamma_1) /| \m{e\_span}(\gamma_1,\tx{x}.\text{L},\gamma_2) /| \m{e\_span}(\gamma_2,\tx{x}.\text{R},\gamma_3)\}$
    } // $\{\exists\gamma_3.~\p{vertices\_at}(R,\gamma_3)/| \gamma(\tx{x}) = (0,\tx{l},\tx{r})  /| \m{mark1}(\gamma, \tx{x}, \gamma_1) /| \m{e\_span}(\gamma_1,\tx{x}.\text{L},\gamma_2) /| \m{e\_span}(\gamma_2,\tx{x}.\text{R},\gamma_3)\}$
} // $\{\exists \gamma_3.~\p{vertex\_at}(\p{reachable}(\gamma, \tx{x}), \gamma_3)/|\m{span}(\gamma,\tx{x},\gamma_3)\}$
\end{lstlisting}

\caption{Clight code and proof sketch for bigraph spanning tree.}
\label{fig:spanning-full}

\end{figure*}
